@prefix rdf:  <http://www.w3.org/1999/02/22-rdf-syntax-ns#> .
@prefix rdfs: <http://www.w3.org/2000/01/rdf-schema#> .
@prefix owl:  <http://www.w3.org/2002/07/owl#> .
@prefix cogsgit: <https://github.com/GSS-Cogs/> .
@prefix cogs: <http://gss-cogs.uk/def/arch/> .

<http://gss-cogs.uk/def/arch> a owl:Ontology;
  rdfs:label "COGS COVID-19 Transform Mapping" ;
.

cogs:SoftwarePackage a owl:Class ;
  rdfs:label "Software package" ;
.
cogs:SoftwarePackage a owl:Class ;
  rdfs:label2 "Label2" ;
.
cogs:LandingPage a owl:Class ;
  rdfs:subClassOf cogs:SoftwarePackage ;
  rdfs:label "Landing Page" ;
.
cogs:Datasets a owl:Class ;
  rdfs:subClassOf cogs:SoftwarePackage ;
  rdfs:label "Output Dataset" ;
.
cogs:Sheets a owl:Class ;
  rdfs:subClassOf cogs:SoftwarePackage ;
  rdfs:label "Sheet Name";
.
cogs:Columns a owl:Class ;
  rdfs:subClassOf cogs:SoftwarePackage ;
  rdfs:label "Table" ;
.
cogs:PMD a owl:Class ;
  rdfs:subClassOf cogs:SoftwarePackage ;
  rdfs:label "PMD" ;
.
cogs:Rename a owl:Class ;
  rdfs:subClassOf cogs:SoftwarePackage ;
  rdfs:label "Rename & Add" ;
.
###########################################################################################################

cogsgit:top-level a cogs:LandingPage ;
  rdfs:label "Landing Page" ;
  rdfs:label2 "<b>Births, Deaths and Other Vital Events - Quarterly Figures for Scotland.</b>" ;
  rdfs:comment <https://www.nrscotland.gov.uk/statistics-and-data/statistics/statistics-by-theme/vital-events/general-publications/births-deaths-and-other-vital-events-quarterly-figures>;
  cogs:scrape cogsgit:sheet1, cogsgit:sheet2, cogsgit:sheet3, cogsgit:sheet4, cogsgit:sheet5, cogsgit:sheet6 ;
.

cogsgit:sheet1 a cogs:Sheets ; rdfs:label "quarter-2-20-tables_Q1_.csv" ; rdfs:comment "Births, stillbirths, deaths, marriages and civil partnerships" ; cogs:transforms cogsgit:dataset1, cogsgit:dataset2 ; .
cogsgit:sheet2 a cogs:Sheets ; rdfs:label "quarter-2-20-tables_Q2_.csv" ; rdfs:comment "Estimated Population, births, stillbirths, deaths, marriages and civil partnerships by admin area" ; cogs:transforms cogsgit:dataset1, cogsgit:dataset2, cogsgit:dataset3 ; .
cogsgit:sheet3 a cogs:Sheets ; rdfs:label "quarter-2-20-tables_Q3_.csv" ; rdfs:comment "Deaths by sex, age and admin area" ; cogs:transforms cogsgit:dataset4 ; .
cogsgit:sheet4 a cogs:Sheets ; rdfs:label "quarter-2-20-tables_Q4_.csv" ; rdfs:comment "Deaths by cause" ; cogs:transforms cogsgit:dataset4 ; .
cogsgit:sheet5 a cogs:Sheets ; rdfs:label "quarter-2-20-tables_Q5_.csv" ; rdfs:comment "Deaths by sex, age and cause" ; cogs:transforms cogsgit:dataset4 ; .
cogsgit:sheet6 a cogs:Sheets ; rdfs:label "quarter-2-20-tables_Q6_.csv" ; rdfs:comment "Deaths by sex, cause and NHS board area" ; cogs:transforms cogsgit:dataset4 ; .

cogsgit:dataset1 a cogs:Rename ; rdfs:label "Dataset One" ; rdfs:comment "Births, deaths, and other vital events, Quarterly figures - Live births, Stillbirths & Perinatal, Neonatal and Infant Deaths<br><br>Numbers and rates" ; cogs:outputs cogsgit:columns1 ; .
cogsgit:dataset2 a cogs:Rename ; rdfs:label "Dataset Two" ; rdfs:comment "Births, deaths, and other vital events, Quarterly figures - Deaths, Marriages & Civil Partnerships<br><br>Numbers and rates" ; cogs:outputs cogsgit:columns2 ; .
cogsgit:dataset3 a cogs:Rename ; rdfs:label "Dataset Three" ; rdfs:comment "Births, deaths, and other vital events, Quarterly figures - Estimated Population by Sex and Council Area" ; cogs:outputs cogsgit:columns3 ; .
cogsgit:dataset4 a cogs:Rename ; rdfs:label "Dataset Four" ; rdfs:comment "Births, deaths, and other vital events, Quarterly figures - Deaths by Age, Sex, Cause of Death and Administrative Area" ; cogs:outputs cogsgit:columns4 ; .

cogsgit:columns1 a cogs:Columns ; rdfs:label "Table" ; rdfs:comment "Period, Vital Event, Sex, Parent Marital Status, Area" ; cogs:uploads cogsgit:pmd1 ; .
cogsgit:columns2 a cogs:Columns ; rdfs:label "Table" ; rdfs:comment "Period, Vital Event, Sex, Area " ; cogs:uploads cogsgit:pmd1 ; .
cogsgit:columns3 a cogs:Columns ; rdfs:label "Table" ; rdfs:comment "Period, Area, Sex, Marker, Values" ; cogs:uploads cogsgit:pmd1 ; .
cogsgit:columns4 a cogs:Columns ; rdfs:label "Table" ; rdfs:comment "Period, Area, Age, Sex, Cause of Death, Values" ; cogs:uploads cogsgit:pmd1 ; .

cogsgit:pmd1 a cogs:PMD ;
  rdfs:label "PMD" ;
  rdfs:comment <https://staging.gss-data.org.uk/datasets?columns=http%3A%2F%2Fpurl.org%2Fdc%2Fterms%2Fpublisher> ;
  .
###################################################################################################
