@prefix rdf:  <http://www.w3.org/1999/02/22-rdf-syntax-ns#> .
@prefix rdfs: <http://www.w3.org/2000/01/rdf-schema#> .
@prefix owl:  <http://www.w3.org/2002/07/owl#> .
@prefix cogsgit: <https://github.com/GSS-Cogs/> .
@prefix cogs: <http://gss-cogs.uk/def/arch/> .

<http://gss-cogs.uk/def/arch> a owl:Ontology;
  rdfs:label "COGS COVID-19 Transform Mapping" ;
.

cogs:SoftwarePackage a owl:Class ;
  rdfs:label "Software package" ;
.
cogs:LandingPage a owl:Class ;
  rdfs:subClassOf cogs:SoftwarePackage ;
  rdfs:label "Landing Page" ;
.
cogs:Datasets a owl:Class ;
  rdfs:subClassOf cogs:SoftwarePackage ;
  rdfs:label "Output Dataset" ;
.
cogs:Sheets a owl:Class ;
  rdfs:subClassOf cogs:SoftwarePackage ;
  rdfs:label "Sheet names to join";
.
cogs:Columns a owl:Class ;
  rdfs:subClassOf cogs:SoftwarePackage ;
  rdfs:label "Table" ;
.
cogs:PMD a owl:Class ;
  rdfs:subClassOf cogs:SoftwarePackage ;
  rdfs:label "PMD" ;
.

###########################################################################################################

cogsgit:top-level a cogs:LandingPage ;
  rdfs:label "Landing Page" ;
  rdfs:label2 "WG NHS activity and capacity during the coronavirus  COVID-19  pandemic";
  rdfs:comment "https://gov.wales/nhs-activity-and-capacity-during-coronavirus-covid-19-pandemic";
  cogs:splits cogsgit:sheet1, cogsgit:sheet2 ;
.

cogsgit:sheet1 a cogs:Sheets ;
  rdfs:label "Sheets" ;
  rdfs:comment "nhs-activity-and-capacity-during-the-coronavirus-covid-19-pandemic-14-may-2020.ods -> Cases_by_LHB, Cases, Deaths, Admissions, Hospitalisations, Critical_Care_Beds, General_and_Acute_Beds, Ambulance_Calls, 111_Calls" ;
  cogs:transforms cogsgit:dataset1 ;
.
cogsgit:sheet2 a cogs:Sheets ;
  rdfs:label "Sheets" ;
  rdfs:comment "a&e-attendances-during-the-coronavirus-covid-19-pandemic-11-may-2020.ods-> A&E_Attendances" ;
  cogs:transforms cogsgit:dataset1 ;
.


cogsgit:dataset1 a cogs:Datasets ;
  rdfs:label "Dataset" ;
  rdfs:comment "WG NHS activity and capacity during the coronavirus COVID-19 pandemic" ;
  cogs:outputs cogsgit:columns1 ;
.


cogsgit:columns1 a cogs:Columns ;
  rdfs:label "Output Table" ;
  rdfs:comment "Period, Local Health Board, Case Count Type, Measure Type, Unit, Marker, Value" ;
  cogs:uploads cogsgit:pmd1 ;
.


cogsgit:pmd1 a cogs:PMD ;
  rdfs:label "PMD" ;
  rdfs:label2 "Publish my Data" ;
  rdfs:comment "http://gss-data.org.uk/data/search" ;
.
###################################################################################################
