@prefix rdf:  <http://www.w3.org/1999/02/22-rdf-syntax-ns#> .
@prefix rdfs: <http://www.w3.org/2000/01/rdf-schema#> .
@prefix owl:  <http://www.w3.org/2002/07/owl#> .
@prefix cogsgit: <https://github.com/GSS-Cogs/> .
@prefix cogs: <http://gss-cogs.uk/def/arch/> .

<http://gss-cogs.uk/def/arch> a owl:Ontology;
  rdfs:label "COGS COVID-19 Transform Mapping" ;
.

cogs:SoftwarePackage a owl:Class ;
  rdfs:label "Software package" ;
.
cogs:SoftwarePackage a owl:Class ;
  rdfs:label2 "Label2" ;
.
cogs:LandingPage a owl:Class ;
  rdfs:subClassOf cogs:SoftwarePackage ;
  rdfs:label "Landing Page" ;
.
cogs:Datasets a owl:Class ;
  rdfs:subClassOf cogs:SoftwarePackage ;
  rdfs:label "Output Dataset" ;
.
cogs:Sheets a owl:Class ;
  rdfs:subClassOf cogs:SoftwarePackage ;
  rdfs:label "Sheet Name";
.
cogs:Columns a owl:Class ;
  rdfs:subClassOf cogs:SoftwarePackage ;
  rdfs:label "Table" ;
.
cogs:PMD a owl:Class ;
  rdfs:subClassOf cogs:SoftwarePackage ;
  rdfs:label "PMD" ;
.
cogs:Rename a owl:Class ;
  rdfs:subClassOf cogs:SoftwarePackage ;
  rdfs:label "Rename & Add" ;
  .

###########################################################################################################

cogsgit:top-level a cogs:LandingPage ;
  rdfs:label "Landing Page" ;
  rdfs:label2 "NISRA Weekly deaths";
  rdfs:comment <https://www.nisra.gov.uk/statistics/ni-summary-statistics/coronavirus-covid-19-statistics>;
  cogs:splits cogsgit:sheet1, cogsgit:sheet2 ;
.

cogsgit:sheet1 a cogs:Sheets ; rdfs:label "Sheets" ; rdfs:label2 "Measures notification date of death" ; rdfs:comment "Table 1, Table 2, Table 3, Table 4, Table 5, Table 6, Table7" ; cogs:transforms cogsgit:dataset1 ; .
cogsgit:sheet2 a cogs:Sheets ; rdfs:label "Sheets" ; rdfs:label2 "Measures actual date of death" ;rdfs:comment "Table 8, Table 9, Table 10, Table 11" ; cogs:transforms cogsgit:dataset2 ; .

cogsgit:dataset1 a cogs:Datasets ; rdfs:label "Output Dataset" ; rdfs:comment "NISRA Weekly Deaths - Notification Date of Death including COVID-19" ; cogs:outputs cogsgit:columns1 ; .
cogsgit:dataset2 a cogs:Datasets ; rdfs:label "Output Dataset" ; rdfs:comment "NISRA Weekly Deaths - Date of Death including COVID-19" ; cogs:outputs cogsgit:columns2 ; .

cogsgit:columns1 a cogs:Columns ; rdfs:label "Table" ; rdfs:comment "Age, Sex, Local Government District, Location of Death, Marker, Measure Type, Period, Registered Death Type, Unit, Value" ; cogs:uploads cogsgit:pmd1; .
cogsgit:columns2 a cogs:Columns ; rdfs:label "Table" ; rdfs:comment "Period, Location of Death, Measure Type, Unit, Marker, Value" ; cogs:uploads cogsgit:pmd1 ; .

cogsgit:pmd1 a cogs:PMD ;
  rdfs:label "Publish my Data" ;
  rdfs:comment <https://staging.gss-data.org.uk/datasets> ;
.


###################################################################################################
