@prefix rdf:  <http://www.w3.org/1999/02/22-rdf-syntax-ns#> .
@prefix rdfs: <http://www.w3.org/2000/01/rdf-schema#> .
@prefix owl:  <http://www.w3.org/2002/07/owl#> .
@prefix cogsgit: <https://github.com/GSS-Cogs/> .
@prefix cogs: <http://gss-cogs.uk/def/arch/> .

<http://gss-cogs.uk/def/arch> a owl:Ontology;
  rdfs:label "COGS COVID-19 Transform Mapping" ;
.

cogs:SoftwarePackage a owl:Class ;
  rdfs:label "Software package" ;
.
cogs:SoftwarePackage a owl:Class ;
  rdfs:label2 "Label2" ;
.
cogs:LandingPage a owl:Class ;
  rdfs:subClassOf cogs:SoftwarePackage ;
  rdfs:label "Landing Page" ;
.
cogs:Datasets a owl:Class ;
  rdfs:subClassOf cogs:SoftwarePackage ;
  rdfs:label "Output Dataset" ;
.
cogs:Sheets a owl:Class ;
  rdfs:subClassOf cogs:SoftwarePackage ;
  rdfs:label "Sheet Name";
.
cogs:Columns a owl:Class ;
  rdfs:subClassOf cogs:SoftwarePackage ;
  rdfs:label "Table" ;
.
cogs:PMD a owl:Class ;
  rdfs:subClassOf cogs:SoftwarePackage ;
  rdfs:label "PMD" ;
.
cogs:Rename a owl:Class ;
  rdfs:subClassOf cogs:SoftwarePackage ;
  rdfs:label "Rename & Add" ;
  .

###########################################################################################################

cogsgit:top-level a cogs:LandingPage ;
  rdfs:label "Landing Page" ;
  rdfs:label2 "NISRA Weekly deaths, Year";
  rdfs:comment "https://www.nisra.gov.uk/statistics/ni-summary-statistics/coronavirus-covid-19-statistics";
  cogs:splits cogsgit:sheet1, cogsgit:sheet2, cogsgit:sheet3, cogsgit:sheet4, cogsgit:sheet5, cogsgit:sheet6, cogsgit:sheet7, cogsgit:sheet8, cogsgit:sheet9 ;
.

cogsgit:sheet1 a cogs:Sheets ; rdfs:label "Weekly Deaths_2020" ; rdfs:comment "Deaths registered each week in Northern Ireland 2020" ; cogs:transforms cogsgit:columns1 ; .
cogsgit:sheet2 a cogs:Sheets ; rdfs:label "Weekly_Deaths_Age by Sex" ; rdfs:comment "Deaths registered each week in Northern Ireland" ; cogs:transforms cogsgit:columns2 ; .
cogsgit:sheet3 a cogs:Sheets ; rdfs:label "Weekly_Deaths_by_LGD" ; rdfs:comment "Deaths registered in Northern Ireland by Local Government District (LGD)" ; cogs:transforms cogsgit:columns3 ; .
cogsgit:sheet4 a cogs:Sheets ; rdfs:label "Covid-19_Deaths_age by sex" ; rdfs:comment "Covid-19 Deaths registered each week in Northern Ireland, age by sex" ; cogs:transforms cogsgit:columns4 ; .
cogsgit:sheet5 a cogs:Sheets ; rdfs:label "Covid-19_Deaths_by_LGD" ; rdfs:comment "Covid-19 Deaths registered in Northern Ireland by Local Government District (LGD)" ; cogs:transforms cogsgit:columns5 ; .
cogsgit:sheet6 a cogs:Sheets ; rdfs:label " Covid-19_Reg Date & POD" ; rdfs:comment "Covid-19 Deaths registered in Northern Ireland by Place of Death" ; cogs:transforms cogsgit:columns6 ; .
cogsgit:sheet7 a cogs:Sheets ; rdfs:label "Covid-19 by Week of Death" ; rdfs:comment " Covid-19 Death Occurrences by week of death in Northern Ireland" ; cogs:transforms cogsgit:columns7 ; .
cogsgit:sheet8 a cogs:Sheets ; rdfs:label " Covid-19 Occurrence Date & POD" ; rdfs:comment "Covid-19 Death Occurrences in Northern Ireland by week of death and Place of Death" ; cogs:transforms cogsgit:columns8 ; .
cogsgit:sheet9 a cogs:Sheets ; rdfs:label "Covid-19 Date of Death & POD" ; rdfs:comment "Covid-19 Death Occurrences by date and Place of Death in Northern Ireland" ; cogs:transforms cogsgit:columns9 ; .


cogsgit:columns1 a cogs:Columns ; rdfs:label "Output Table 1" ; rdfs:comment "Registration Week, Week Ending, Registered Death Type, Measure Type, Unit, Marker, Value" ; cogs:harmonise cogsgit:rename1 ; .
cogsgit:columns2 a cogs:Columns ; rdfs:label "Output Table 2" ; rdfs:comment "Gender, Age, Week Number, Week Ending, Measure Type, Unit, Marker, Value" ; cogs:harmonise cogsgit:rename2 ; .
cogsgit:columns3 a cogs:Columns ; rdfs:label "Output Table 3" ; rdfs:comment "Registration Week, Week Ending, Local Government District, Measure Type, Unit, Marker, Value" ; cogs:harmonise cogsgit:rename3 ; .
cogsgit:columns4 a cogs:Columns ; rdfs:label "Output Table 4" ; rdfs:comment "Gender, Age, Week Number, Week Ending, Measure Type, Unit, Marker, Value" ; cogs:harmonise cogsgit:rename4 ; .
cogsgit:columns5 a cogs:Columns ; rdfs:label "Output Table 5" ; rdfs:comment "Registration Week, Week Ending, Local Government District, Measure Type, Unit, Marker, Value" ; cogs:harmonise cogsgit:rename5 ; .
cogsgit:columns6 a cogs:Columns ; rdfs:label "Output Table 6" ; rdfs:comment "Week of Death, Week Ending, Place of Death, Measure Type, Unit, Marker, Value" ; cogs:harmonise cogsgit:rename6 ; .
cogsgit:columns7 a cogs:Columns ; rdfs:label "Output Table 7" ; rdfs:comment "Week of Death, Week Ending, COVID-19 Deaths, Measure Type, Unit, Marker, Value" ; cogs:harmonise cogsgit:rename7 ; .
cogsgit:columns8 a cogs:Columns ; rdfs:label "Output Table 8" ; rdfs:comment "Week of Death, Week Ending, Place of Death, Measure Type, Unit, Marker, Value" ; cogs:harmonise cogsgit:rename8 ; .
cogsgit:columns9 a cogs:Columns ; rdfs:label "Output Table 9" ; rdfs:comment "Date, Place of Death, Measure Type, Unit, Marker, Value" ; cogs:harmonise cogsgit:rename9 ; .


cogsgit:rename1 a cogs:Rename ; rdfs:label "Rename & Add" ; rdfs:comment "Not yet specified" ; cogs:joins cogsgit:dataset1 ; .
cogsgit:rename2 a cogs:Rename ; rdfs:label "Rename & Add" ; rdfs:comment "Not yet specified" ; cogs:joins cogsgit:dataset1 ; .
cogsgit:rename3 a cogs:Rename ; rdfs:label "Rename & Add" ; rdfs:comment "Not yet specified" ; cogs:joins cogsgit:dataset1 ; .
cogsgit:rename4 a cogs:Rename ; rdfs:label "Rename & Add" ; rdfs:comment "Not yet specified" ; cogs:joins cogsgit:dataset1 ; .
cogsgit:rename5 a cogs:Rename ; rdfs:label "Rename & Add" ; rdfs:comment "Not yet specified" ; cogs:joins cogsgit:dataset1 ; .
cogsgit:rename6 a cogs:Rename ; rdfs:label "Rename & Add" ; rdfs:comment "Not yet specified" ; cogs:joins cogsgit:dataset1 ; .
cogsgit:rename7 a cogs:Rename ; rdfs:label "Rename & Add" ; rdfs:comment "Not yet specified" ; cogs:joins cogsgit:dataset1 ; .
cogsgit:rename8 a cogs:Rename ; rdfs:label "Rename & Add" ; rdfs:comment "Not yet specified" ; cogs:joins cogsgit:dataset1 ; .
cogsgit:rename9 a cogs:Rename ; rdfs:label "Rename & Add" ; rdfs:comment "Not yet specified" ; cogs:joins cogsgit:dataset1 ; .


cogsgit:dataset1 a cogs:Datasets ; rdfs:label "Dataset Name 1" ; rdfs:comment "Dataset Name" ; cogs:outputs cogsgit:pmd1 ; .

cogsgit:pmd1 a cogs:PMD ;
  rdfs:label "PMD" ;
  rdfs:comment "Publish my Data: http://gss-data.org.uk/data/search" ;
.
###################################################################################################
