@prefix rdf:  <http://www.w3.org/1999/02/22-rdf-syntax-ns#> .
@prefix rdfs: <http://www.w3.org/2000/01/rdf-schema#> .
@prefix owl:  <http://www.w3.org/2002/07/owl#> .
@prefix cogsgit: <https://github.com/GSS-Cogs/> .
@prefix cogs: <http://gss-cogs.uk/def/arch/> .

<http://gss-cogs.uk/def/arch> a owl:Ontology;
  rdfs:label "COGS COVID-19 Transform Mapping" ;
.

cogs:SoftwarePackage a owl:Class ;
  rdfs:label "Software package" ;
.
cogs:SoftwarePackage a owl:Class ;
  rdfs:label2 "Label2" ;
.
cogs:LandingPage a owl:Class ;
  rdfs:subClassOf cogs:SoftwarePackage ;
  rdfs:label "Landing Page" ;
.
cogs:Datasets a owl:Class ;
  rdfs:subClassOf cogs:SoftwarePackage ;
  rdfs:label "Output Dataset" ;
.
cogs:Sheets a owl:Class ;
  rdfs:subClassOf cogs:SoftwarePackage ;
  rdfs:label "Sheet Name";
.
cogs:Columns a owl:Class ;
  rdfs:subClassOf cogs:SoftwarePackage ;
  rdfs:label "Table" ;
.
cogs:PMD a owl:Class ;
  rdfs:subClassOf cogs:SoftwarePackage ;
  rdfs:label "PMD" ;
.
cogs:Rename a owl:Class ;
  rdfs:subClassOf cogs:SoftwarePackage ;
  rdfs:label "Rename & Add" ;
  .

###########################################################################################################

cogsgit:top-level a cogs:LandingPage ;
  rdfs:label "Landing Page" ;
  rdfs:label2 "Deaths involving COVID-19 in the care sector, England and Wales";
  rdfs:comment <https://www.ons.gov.uk/peoplepopulationandcommunity/birthsdeathsandmarriages/deaths/datasets/deathsinvolvingcovid19inthecaresectorenglandandwales>;
  cogs:splits cogsgit:sheet1 ;
.

cogsgit:sheet1 a cogs:Sheets ; rdfs:label "Sheets" ; rdfs:label2 "Measures Deaths in the care sector from 3 sources (ONS, CQC, CIW)" ; rdfs:comment "Table 1, Table 2, Table 5, Table 6, Table 7, Table 8, Table 9, Table 10, Table 11, Table 12, Table 13, Table 14, Table 15, Table 16" ; cogs:transforms cogsgit:dataset1 ; .
cogsgit:sheet2 a cogs:Sheets ; rdfs:label "Sheets" ; rdfs:label2 "Measures Age standardised mortality rates by Age & Sex" ; rdfs:comment "Table 3, Table 4" ; cogs:transforms cogsgit:dataset2 ; .
cogsgit:sheet3 a cogs:Sheets ; rdfs:label "Sheets" ; rdfs:label2 "Measures Deaths by leading cause groupings" ; rdfs:comment "Table 17" ; cogs:transforms cogsgit:dataset3 ; .
cogsgit:sheet4 a cogs:Sheets ; rdfs:label "Sheets" ; rdfs:label2 "Measures proportion of deaths Deaths from COVID-19 by main pre-existing condition" ; rdfs:comment "Table 18" ; cogs:transforms cogsgit:dataset4 ; .

cogsgit:dataset1 a cogs:Datasets ; rdfs:label "Output Dataset" ; rdfs:comment "Deaths involving COVID-19 in the care sector for England and Wales" ; cogs:outputs cogsgit:columns1 ; .
cogsgit:dataset2 a cogs:Datasets ; rdfs:label "Output Dataset" ; rdfs:comment "Deaths in the care sector for England and Wales - Age standardised mortality rates by Age & Sex" ; cogs:outputs cogsgit:columns2 ; .
cogsgit:dataset3 a cogs:Datasets ; rdfs:label "Output Dataset" ; rdfs:comment "Deaths in the care sector for England and Wales by leading cause groupings" ; cogs:outputs cogsgit:columns3 ; .
cogsgit:dataset4 a cogs:Datasets ; rdfs:label "Output Dataset" ; rdfs:comment "Proportion of Deaths in the care sector for England and Wales by main pre-existing condition" ; cogs:outputs cogsgit:columns4 ; .

cogsgit:columns1 a cogs:Columns ; rdfs:label "Table" ; rdfs:comment "Period, Recorded Death Type, Source, Person Type, Sex, Age, Area, Place of death, Cause of death, Measure Type, Unit, Value" ; cogs:uploads cogsgit:pmd1; .
cogsgit:columns2 a cogs:Columns ; rdfs:label "Table" ; rdfs:comment "Period, Recorded Death Type, Source, Cause of death, Sex, Age, Local Authority, Person Type, Lower 95% CI, Upper 95% CI, Number of deaths, Measure Type, Unit, Value" ; cogs:uploads cogsgit:pmd1; .
cogsgit:columns3 a cogs:Columns ; rdfs:label "Table" ; rdfs:comment "Period, Leading cause of Death, Sex, Area, Measure Type, Unit, Value" ; cogs:uploads cogsgit:pmd1; .
cogsgit:columns4 a cogs:Columns ; rdfs:label "Table" ; rdfs:comment "Period, Main Pre-existing Condition, Sex, Age, Local Authority, Measure Type, Unit, Value" ; cogs:uploads cogsgit:pmd1; .

cogsgit:pmd1 a cogs:PMD ;
  rdfs:label "Publish my Data" ;
  rdfs:comment <https://staging.gss-data.org.uk/datasets> ;
.


###################################################################################################
