@prefix rdf:  <http://www.w3.org/1999/02/22-rdf-syntax-ns#> .
@prefix rdfs: <http://www.w3.org/2000/01/rdf-schema#> .
@prefix owl:  <http://www.w3.org/2002/07/owl#> .
@prefix cogsgit: <https://github.com/GSS-Cogs/> .
@prefix cogs: <http://gss-cogs.uk/def/arch/> .

<http://gss-cogs.uk/def/arch> a owl:Ontology;
  rdfs:label "COGS COVID-19 Transform Mapping" ;
.

cogs:SoftwarePackage a owl:Class ;
  rdfs:label "Software package" ;
.
cogs:LandingPage a owl:Class ;
  rdfs:subClassOf cogs:SoftwarePackage ;
  rdfs:label "Landing Page" ;
.
cogs:Datasets a owl:Class ;
  rdfs:subClassOf cogs:SoftwarePackage ;
  rdfs:label "Output Dataset" ;
.
cogs:Sheets a owl:Class ;
  rdfs:subClassOf cogs:SoftwarePackage ;
  rdfs:label "Sheet Name";
.
cogs:Columns a owl:Class ;
  rdfs:subClassOf cogs:SoftwarePackage ;
  rdfs:label "Table" ;
.
cogs:PMD a owl:Class ;
  rdfs:subClassOf cogs:SoftwarePackage ;
  rdfs:label "PMD" ;
.
cogs:Rename a owl:Class ;
  rdfs:subClassOf cogs:SoftwarePackage ;
  rdfs:label "Rename & Add" ;
.
###########################################################################################################

cogsgit:top-level a cogs:LandingPage ;
  rdfs:label "Landing Page" ;
  rdfs:comment "Notifications of deaths of residents related to COVID-19 in adult care homes \n https://gov.wales/notifications-deaths-residents-related-covid-19-adult-care-homes";
  cogs:scrape cogsgit:sheet1, cogsgit:sheet2, cogsgit:sheet3, cogsgit:sheet4, cogsgit:sheet5, cogsgit:sheet6, cogsgit:sheet7, cogsgit:sheet8, cogsgit:sheet9 ;
.

cogsgit:sheet1 a cogs:Sheets ; rdfs:label "Table_1" ; rdfs:comment "Notifications of Service User Deaths received from Adult Care Homes" ; cogs:transforms cogsgit:columns1 ; .
cogsgit:sheet2 a cogs:Sheets ; rdfs:label "Table_2" ; rdfs:comment "Notifications of deaths of adult care home residents with confirmed or suspected COVID-19 by location of death" ; cogs:transforms cogsgit:columns2 ; .
cogsgit:sheet3 a cogs:Sheets ; rdfs:label "Table_3" ; rdfs:comment "Notifications of deaths of residents from adult care homes by date of notification and cause" ; cogs:transforms cogsgit:columns3 ; .
cogsgit:sheet4 a cogs:Sheets ; rdfs:label "Table_4" ; rdfs:comment "Notifications of deaths of adult care home residents with confirmed or suspected covid-19 by location of death and date of notification" ; cogs:transforms cogsgit:columns4 ; .
cogsgit:sheet5 a cogs:Sheets ; rdfs:label "Table_5" ; rdfs:comment "Notifications of deaths of adult care home residents by location of death and date of notification" ; cogs:transforms cogsgit:columns5 ; .
cogsgit:sheet6 a cogs:Sheets ; rdfs:label "Table_6" ; rdfs:comment "Number of notifications of deaths of adult care home residents involving COVID-19 (both confirmed and suspected) occurring in care homes, by Local Authority and day of notification" ; cogs:transforms cogsgit:columns6 ; .
cogsgit:sheet7 a cogs:Sheets ; rdfs:label "Table_7" ; rdfs:comment "Number of notifications of deaths of adult care home residents involving COVID-19 (both confirmed and suspected) occurring in any location, by Local Authority and day of notification" ; cogs:transforms cogsgit:columns7 ; .
cogsgit:sheet8 a cogs:Sheets ; rdfs:label "Table_8" ; rdfs:comment "Number of notifications of deaths of adult care home residents by Local Authority and day of notification" ; cogs:transforms cogsgit:columns8 ;.
cogsgit:sheet9 a cogs:Sheets ; rdfs:label "Table_9" ; rdfs:comment "Number of notifications of deaths of adult care home residents occurring in care homes by Local Authority and day of notification" ; cogs:transforms cogsgit:columns9 ; .


cogsgit:columns1 a cogs:Columns ; rdfs:label "Output Table 1" ; rdfs:comment "Notification Date Range, Care Provided, Measure Type, Unit, Marker, Value" ; cogs:harmonise cogsgit:rename1 ; .
cogsgit:columns2 a cogs:Columns ; rdfs:label "Output Table 2" ; rdfs:comment "Notification Date Range, Location of Death, Measure Type, Unit, Marker, Value" ; cogs:harmonise cogsgit:rename2 ; .
cogsgit:columns3 a cogs:Columns ; rdfs:label "Output Table 3" ; rdfs:comment "Notification Day, Notification Year, Cause of Death, Measure Type, Unit, Marker, Value" ; cogs:harmonise cogsgit:rename3 ; .
cogsgit:columns4 a cogs:Columns ; rdfs:label "Output Table 4" ; rdfs:comment "Notification Date, Location of Death, Measure Type, Unit, Marker, Value" ; cogs:harmonise cogsgit:rename4 ; .
cogsgit:columns5 a cogs:Columns ; rdfs:label "Output Table 5" ; rdfs:comment "Notification Date, Location of Death, Measure Type, Unit, Marker, Value" ; cogs:harmonise cogsgit:rename5 ; .
cogsgit:columns6 a cogs:Columns ; rdfs:label "Output Table 6" ; rdfs:comment "Area Code, Local Authority, Notification Date, Measure Type, Unit, Marker, Value" ; cogs:harmonise cogsgit:rename6 ; .
cogsgit:columns7 a cogs:Columns ; rdfs:label "Output Table 7" ; rdfs:comment "Area Code, Local Authority, Notification Date, Measure Type, Unit, Marker, Value" ; cogs:harmonise cogsgit:rename7 ; .
cogsgit:columns8 a cogs:Columns ; rdfs:label "Output Table 8" ; rdfs:comment "Area Code, Local Authority, Notification Date, Measure Type, Unit, Marker, Value" ; cogs:harmonise cogsgit:rename8 ; .
cogsgit:columns9 a cogs:Columns ; rdfs:label "Output Table 9" ; rdfs:comment "Area Code, Local Authority, Notification Date, Measure Type, Unit, Marker, Value" ; cogs:harmonise cogsgit:rename9 ; .


cogsgit:rename1 a cogs:Rename ; rdfs:label "Rename & Add" ; rdfs:comment "Rename 1" ; cogs:joins cogsgit:dataset1 ; .
cogsgit:rename2 a cogs:Rename ; rdfs:label "Rename & Add" ; rdfs:comment "Rename 2" ; cogs:joins cogsgit:dataset2 ; .
cogsgit:rename3 a cogs:Rename ; rdfs:label "Rename & Add" ; rdfs:comment "Rename 3" ; cogs:joins cogsgit:dataset2 ; .
cogsgit:rename4 a cogs:Rename ; rdfs:label "Rename & Add" ; rdfs:comment "Rename 4" ; cogs:joins cogsgit:dataset2 ; .
cogsgit:rename5 a cogs:Rename ; rdfs:label "Rename & Add" ; rdfs:comment "Rename 5" ; cogs:joins cogsgit:dataset2 ; .
cogsgit:rename6 a cogs:Rename ; rdfs:label "Rename & Add" ; rdfs:comment "Rename 6" ; cogs:joins cogsgit:dataset2 ; .
cogsgit:rename7 a cogs:Rename ; rdfs:label "Rename & Add" ; rdfs:comment "Rename 7" ; cogs:joins cogsgit:dataset2 ; .
cogsgit:rename8 a cogs:Rename ; rdfs:label "Rename & Add" ; rdfs:comment "Rename 8" ; cogs:joins cogsgit:dataset2 ; .
cogsgit:rename9 a cogs:Rename ; rdfs:label "Rename & Add" ; rdfs:comment "Rename 9" ; cogs:joins cogsgit:dataset2 ; .


cogsgit:dataset1 a cogs:Datasets ; rdfs:label "Dataset Name 1" ; rdfs:comment "Dataset 1" ; cogs:outputs cogsgit:pmd1 ; .
cogsgit:dataset2 a cogs:Datasets ; rdfs:label "Dateset Name 2" ; rdfs:comment "Dataset 2" ; cogs:outputs cogsgit:pmd1 ; .


cogsgit:pmd1 a cogs:PMD ;
  rdfs:label "" ;
  rdfs:comment "Publish my Data: http://gss-data.org.uk/data/search" ;
.
###################################################################################################
