@prefix rdf:  <http://www.w3.org/1999/02/22-rdf-syntax-ns#> .
@prefix rdfs: <http://www.w3.org/2000/01/rdf-schema#> .
@prefix owl:  <http://www.w3.org/2002/07/owl#> .
@prefix cogsgit: <https://github.com/GSS-Cogs/> .
@prefix cogs: <http://gss-cogs.uk/def/arch/> .

<http://gss-cogs.uk/def/arch> a owl:Ontology;
  rdfs:label "COGS COVID-19 Transform Mapping" ;
.

cogs:SoftwarePackage a owl:Class ;
  rdfs:label "Software package" ;
.
cogs:LandingPage a owl:Class ;
  rdfs:subClassOf cogs:SoftwarePackage ;
  rdfs:label "Landing Page" ;
.
cogs:Datasets a owl:Class ;
  rdfs:subClassOf cogs:SoftwarePackage ;
  rdfs:label "Output Dataset" ;
.
cogs:Sheets a owl:Class ;
  rdfs:subClassOf cogs:SoftwarePackage ;
  rdfs:label "Sheet names to join";
.
cogs:Columns a owl:Class ;
  rdfs:subClassOf cogs:SoftwarePackage ;
  rdfs:label "Table" ;
.
cogs:PMD a owl:Class ;
  rdfs:subClassOf cogs:SoftwarePackage ;
  rdfs:label "PMD" ;
.

###########################################################################################################

cogsgit:top-level a cogs:LandingPage ;
  rdfs:label "Notifications of deaths of residents related to COVID-19 in adult care homes" ;
  rdfs:comment "https://gov.wales/notifications-deaths-residents-related-covid-19-adult-care-homes";
  cogs:splits cogsgit:sheet1, cogsgit:sheet2, cogsgit:sheet3, cogsgit:sheet4, cogsgit:sheet5, cogsgit:sheet6, cogsgit:sheet7, cogsgit:sheet8, cogsgit:sheet9 ;
.

cogsgit:sheet1 a cogs:Sheets ; rdfs:label "" ; rdfs:comment "Table_1 Notifications of Service User Deaths received from Adult Care Homes" ; cogs:transforms cogsgit:columns1 ; .
cogsgit:sheet2 a cogs:Sheets ; rdfs:label "" ; rdfs:comment "Table_2 Notifications of deaths of adult care home residents with confirmed or suspected COVID-19 by location of death" ; cogs:transforms cogsgit:columns2 ; .
cogsgit:sheet3 a cogs:Sheets ; rdfs:label "" ; rdfs:comment "Table_3 Notifications of deaths of residents from adult care homes by date of notification and cause" ; cogs:transforms cogsgit:columns3 ; .
cogsgit:sheet4 a cogs:Sheets ; rdfs:label "" ; rdfs:comment "Table_4 Notifications of deaths of adult care home residents with confirmed or suspected covid-19 by location of death and date of notification" ; cogs:transforms cogsgit:columns4 ; .
cogsgit:sheet5 a cogs:Sheets ; rdfs:label "" ; rdfs:comment "Table_5 Notifications of deaths of adult care home residents by location of death and date of notification" ; cogs:transforms cogsgit:columns5 ; .
cogsgit:sheet6 a cogs:Sheets ; rdfs:label "" ; rdfs:comment "Table_6 Number of notifications of deaths of adult care home residents involving COVID-19 (both confirmed and suspected) occurring in care homes, by Local Authority and day of notification" ; cogs:transforms cogsgit:columns6 ; .
cogsgit:sheet7 a cogs:Sheets ; rdfs:label "" ; rdfs:comment "Table_7 Number of notifications of deaths of adult care home residents involving COVID-19 (both confirmed and suspected) occurring in any location, by Local Authority and day of notification" ; cogs:transforms cogsgit:columns7 ; .
cogsgit:sheet8 a cogs:Sheets ; rdfs:label "" ; rdfs:comment "Table_8 Number of notifications of deaths of adult care home residents by Local Authority and day of notification" ; cogs:transforms cogsgit:columns8 ; .
cogsgit:sheet9 a cogs:Sheets ; rdfs:label "" ; rdfs:comment "Table_9 Number of notifications of deaths of adult care home residents occurring in care homes by Local Authority and day of notification" ; cogs:transforms cogsgit:columns9 ; .


cogsgit:columns1 a cogs:Columns ; rdfs:label "" ; rdfs:comment "Notification Date Range, Care Provided, Measure Type, Unit, Marker, Value" ; .
cogsgit:columns2 a cogs:Columns ; rdfs:label "" ; rdfs:comment "Notification Date Range, Location of Death, Measure Type, Unit, Marker, Value" ; .
cogsgit:columns3 a cogs:Columns ; rdfs:label "" ; rdfs:comment "Notification Day, Notification Year, Cause of Death, Measure Type, Unit, Marker, Value" ; .
cogsgit:columns4 a cogs:Columns ; rdfs:label "" ; rdfs:comment "Notification Date, Location of Death, Measure Type, Unit, Marker, Value" ; .
cogsgit:columns5 a cogs:Columns ; rdfs:label "" ; rdfs:comment "Notification Date, Location of Death, Measure Type, Unit, Marker, Value" ; .
cogsgit:columns6 a cogs:Columns ; rdfs:label "" ; rdfs:comment "Area Code, Local Authority, Notification Date, Measure Type, Unit, Marker, Value" ; .
cogsgit:columns7 a cogs:Columns ; rdfs:label "" ; rdfs:comment "Area Code, Local Authority, Notification Date, Measure Type, Unit, Marker, Value" ; .
cogsgit:columns8 a cogs:Columns ; rdfs:label "" ; rdfs:comment "Area Code, Local Authority, Notification Date, Measure Type, Unit, Marker, Value" ; .
cogsgit:columns9 a cogs:Columns ; rdfs:label "" ; rdfs:comment "Area Code, Local Authority, Notification Date, Measure Type, Unit, Marker, Value" ; .


###################################################################################################
