@prefix rdf:  <http://www.w3.org/1999/02/22-rdf-syntax-ns#> .
@prefix rdfs: <http://www.w3.org/2000/01/rdf-schema#> .
@prefix owl:  <http://www.w3.org/2002/07/owl#> .
@prefix cogsgit: <https://github.com/GSS-Cogs/> .
@prefix cogs: <http://gss-cogs.uk/def/arch/> .

<http://gss-cogs.uk/def/arch> a owl:Ontology;
  rdfs:label "COGS COVID-19 Transform Mapping" ;
.

cogs:SoftwarePackage a owl:Class ;
  rdfs:label "Software package" ;
.
cogs:LandingPage a owl:Class ;
  rdfs:subClassOf cogs:SoftwarePackage ;
  rdfs:label "Landing Page" ;
.
cogs:Datasets a owl:Class ;
  rdfs:subClassOf cogs:SoftwarePackage ;
  rdfs:label "Output Dataset" ;
.
cogs:Sheets a owl:Class ;
  rdfs:subClassOf cogs:SoftwarePackage ;
  rdfs:label "Sheet names to join";
.
cogs:Columns a owl:Class ;
  rdfs:subClassOf cogs:SoftwarePackage ;
  rdfs:label "Table" ;
.
cogs:PMD a owl:Class ;
  rdfs:subClassOf cogs:SoftwarePackage ;
  rdfs:label "PMD" ;
.

###########################################################################################################

cogsgit:top-level a cogs:LandingPage ;
  rdfs:label "Landing Page" ;
  rdfs:comment "<b>WG Summary data about coronavirus  COVID-19  and the response to it </b> \n https://gov.wales/summary-data-about-coronavirus-covid-19-and-response-it";
  cogs:splits cogsgit:sheet1, cogsgit:sheet2 ;
.

cogsgit:sheet1 a cogs:Sheets ;
  rdfs:label "Sheets" ;
  rdfs:comment "Food Parcels" ;
  cogs:transforms cogsgit:dataset1 ;
.
cogsgit:sheet2 a cogs:Sheets ;
  rdfs:label "Sheets" ;
  rdfs:comment "Discretionary_Assistance_Fund, Business_Rates_Grants, Business_Rates_Grants, DBW_loans, ERF" ;
  cogs:transforms cogsgit:dataset2 ;
.


cogsgit:dataset1 a cogs:Datasets ;
  rdfs:label "Dataset" ;
  rdfs:comment "WG COVID-19 Food Parcel Support" ;
  cogs:outputs cogsgit:columns1 ;
.
cogsgit:dataset2 a cogs:Datasets ;
  rdfs:label "Dataset" ;
  rdfs:comment "WG COVID-19 Support Response" ;
  cogs:outputs cogsgit:columns2 ;
.


cogsgit:columns1 a cogs:Columns ;
  rdfs:label "Output Table" ;
  rdfs:comment "Period, Food Parcel Status, Measure Type, Unit, Marker, Value" ;
  cogs:uploads cogsgit:pmd1 ;
.
cogsgit:columns2 a cogs:Columns ;
  rdfs:label "" ;
  rdfs:comment "Period, Support Type, Finance Type, Measure Type, Unit, Marker, Value" ;
  cogs:uploads cogsgit:pmd1 ;
.


cogsgit:pmd1 a cogs:PMD ;
  rdfs:label "PMD" ;
  rdfs:comment "Publish my Data: http://gss-data.org.uk/data/search" ;
.
###################################################################################################
