@prefix rdf:  <http://www.w3.org/1999/02/22-rdf-syntax-ns#> .
@prefix rdfs: <http://www.w3.org/2000/01/rdf-schema#> .
@prefix owl:  <http://www.w3.org/2002/07/owl#> .
@prefix cogsgit: <https://github.com/GSS-Cogs/> .
@prefix cogs: <http://gss-cogs.uk/def/arch/> .

<http://gss-cogs.uk/def/arch> a owl:Ontology;
  rdfs:label "COGS COVID-19 Transform Mapping" ;
.

cogs:SoftwarePackage a owl:Class ;
  rdfs:label "Software package" ;
.
cogs:SoftwarePackage a owl:Class ;
  rdfs:label2 "Label2" ;
.
cogs:LandingPage a owl:Class ;
  rdfs:subClassOf cogs:SoftwarePackage ;
  rdfs:label "Landing Page" ;
.
cogs:Datasets a owl:Class ;
  rdfs:subClassOf cogs:SoftwarePackage ;
  rdfs:label "Output Dataset" ;
.
cogs:Sheets a owl:Class ;
  rdfs:subClassOf cogs:SoftwarePackage ;
  rdfs:label "Sheet Name";
.
cogs:Columns a owl:Class ;
  rdfs:subClassOf cogs:SoftwarePackage ;
  rdfs:label "Table" ;
.
cogs:PMD a owl:Class ;
  rdfs:subClassOf cogs:SoftwarePackage ;
  rdfs:label "PMD" ;
.
cogs:Rename a owl:Class ;
  rdfs:subClassOf cogs:SoftwarePackage ;
  rdfs:label "Rename & Add" ;
.
###########################################################################################################

cogsgit:top-level a cogs:LandingPage ;
  rdfs:label "Landing Page" ;
  rdfs:label2 "<b>NHS D Coronavirus Shielded Patient List Summary Totals, England</b>" ;
  rdfs:comment "https://digital.nhs.uk/data-and-information/publications/statistical/mi-english-coronavirus-covid-19-shielded-patient-list-summary-totals/latest";
  cogs:scrape cogsgit:sheet1, cogsgit:sheet2 ;
.

cogsgit:sheet1 a cogs:Sheets ; rdfs:label "Stage 1: Transform" ; rdfs:comment "Filename: Coronavirus Shielded Patient List, England - Open Data - CCG<br>Sheets: Coronavirus Shielded Patient Li" ; cogs:transforms cogsgit:columns1 ; .
cogsgit:sheet2 a cogs:Sheets ; rdfs:label "Stage 1: Transform" ; rdfs:comment "Filename: Coronavirus Shielded Patient List, England - Open Data - LA<br>Sheets: Coronavirus Shielded Patient Li" ; cogs:transforms cogsgit:columns2 ; .


cogsgit:columns1 a cogs:Columns ; rdfs:label "Output Table 1" ; rdfs:comment "Extract Date, CCG Code, CCG Name, Breakdown Field, Breakdown Value, Patient Count, Measure Type, Unit, Marker, Value" ; cogs:harmonise cogsgit:rename1 ; .
cogsgit:columns2 a cogs:Columns ; rdfs:label "Output Table 2" ; rdfs:comment "Extract Date, LA Code, LA Name, Breakdown Field, Breakdown Value, Patient Count, Measure Type, Unit, Marker, Value" ; cogs:harmonise cogsgit:rename2 ; .


cogsgit:rename1 a cogs:Rename ; rdfs:label "Stage 2: Harmonise" ; rdfs:comment "Not yet defined" ; cogs:joins cogsgit:dataset1 ; .
cogsgit:rename2 a cogs:Rename ; rdfs:label "Stage 2: Harmonise" ; rdfs:comment "Not yet defined" ; cogs:joins cogsgit:dataset1 ; .


cogsgit:dataset1 a cogs:Datasets ; rdfs:label "Dataset Name 1" ; rdfs:comment "Not yet defined" ; cogs:outputs cogsgit:pmd1 ; .

cogsgit:pmd1 a cogs:PMD ;
  rdfs:label "PMD" ;
  rdfs:comment "Publish my Data: http://gss-data.org.uk/data/search" ;
.
###################################################################################################
