@prefix rdf:  <http://www.w3.org/1999/02/22-rdf-syntax-ns#> .
@prefix rdfs: <http://www.w3.org/2000/01/rdf-schema#> .
@prefix owl:  <http://www.w3.org/2002/07/owl#> .
@prefix cogsgit: <https://github.com/GSS-Cogs/> .
@prefix cogs: <http://gss-cogs.uk/def/arch/> .

<http://gss-cogs.uk/def/arch> a owl:Ontology;
  rdfs:label "COGS COVID-19 Transform Mapping" ;
.

cogs:SoftwarePackage a owl:Class ;
  rdfs:label "Software package" ;
.
cogs:SoftwarePackage a owl:Class ;
  rdfs:label2 "Label2" ;
.
cogs:LandingPage a owl:Class ;
  rdfs:subClassOf cogs:SoftwarePackage ;
  rdfs:label "Landing Page" ;
.
cogs:Datasets a owl:Class ;
  rdfs:subClassOf cogs:SoftwarePackage ;
  rdfs:label "Output Dataset" ;
.
cogs:Sheets a owl:Class ;
  rdfs:subClassOf cogs:SoftwarePackage ;
  rdfs:label "Sheet Name";
.
cogs:Columns a owl:Class ;
  rdfs:subClassOf cogs:SoftwarePackage ;
  rdfs:label "Table" ;
.
cogs:PMD a owl:Class ;
  rdfs:subClassOf cogs:SoftwarePackage ;
  rdfs:label "PMD" ;
.
cogs:Rename a owl:Class ;
  rdfs:subClassOf cogs:SoftwarePackage ;
  rdfs:label "Rename & Add" ;
.
###########################################################################################################

cogsgit:top-level a cogs:LandingPage ;
  rdfs:label "Landing Page" ;
  rdfs:label2 "<b>Which occupations have the highest potential exposure to the coronavirus (COVID-19)?</b>" ;
  rdfs:comment <https://www.ons.gov.uk/employmentandlabourmarket/peopleinwork/employmentandemployeetypes/articles/whichoccupationshavethehighestpotentialexposuretothecoronaviruscovid19/2020-05-11>;
  cogs:scrape cogsgit:sheet1, cogsgit:sheet2 ;
.

cogsgit:sheet1 a cogs:Sheets ; rdfs:label "Sheet" ; rdfs:comment "Occupations and exposure" ; cogs:transforms cogsgit:dataset1 ; .
cogsgit:sheet2 a cogs:Sheets ; rdfs:label "Sheet" ; rdfs:comment "Total workforce population" ; cogs:transforms cogsgit:dataset2 ; .


cogsgit:dataset1 a cogs:Datasets ; rdfs:label "Dataset 1" ; rdfs:comment "Which occupations have the highest potential exposure to the coronavirus COVID-19" ; cogs:outputs cogsgit:columns1 ; .
cogsgit:dataset2 a cogs:Datasets ; rdfs:label "Dataset 2" ; rdfs:comment "Which occupations have the highest potential exposure to the coronavirus COVID-19 - Total Workforce Population" ; cogs:outputs cogsgit:columns2 ; .


cogsgit:columns1 a cogs:Columns ; rdfs:label "Output Table 1" ; rdfs:comment "UK SOC 2010 Code, Occupation, Total in employment, Median hourly pay, Percentage Workforce Female, Percentage Workforce Aged 55plus, Percentage Workforce BAME, Working Condition Category, Measure type, Unit, Value" ; cogs:uploads cogsgit:PMD1 ; .
cogsgit:columns2 a cogs:Columns ; rdfs:label "Output Table 2" ; rdfs:comment "Workforce Category, Measure Type, Unit, Value" ; cogs:uploads cogsgit:PMD1 ; .


cogsgit:pmd1 a cogs:PMD ; rdfs:label "PMD" ; rdfs:comment <https://staging.gss-data.org.uk/datasets> ; .
###################################################################################################
